lib/Literal.lean
@@ -1,13 +1,148 @@
-import RDF
+import lib.NamedNode
+import lib.vocab
+import LeanCopilot
 
-instance : Coe Int Literal where
-  coe s := Literal.DataTyped (toString s) "http://www.w3.org/2001/XMLSchema#integer"
+structure LanguageTaggedStringLiteral where
+  value : String
+  language : String
+deriving Repr, BEq
 
-instance : Coe Bool Literal where
-  coe s := Literal.DataTyped (toString s) "http://www.w3.org/2001/XMLSchema#boolean"
+structure TypedLiteral where
+  value : String
+  datatype : NamedNode
+deriving Repr, BEq
 
-instance : Coe Float Literal where
-  coe s := Literal.DataTyped (toString s) "http://www.w3.org/2001/XMLSchema#float"
+inductive Literal where
+  | LanguageTaggedString : LanguageTaggedStringLiteral → Literal
+  | Typed : TypedLiteral → Literal
+deriving Repr, BEq
 
-instance : Coe String Literal where
-  coe s := Literal.DataTyped s "http://www.w3.org/2001/XMLSchema#string"
+def Literal.toTyped? : Literal → (Option TypedLiteral)
+  | Literal.Typed l => some l
+  | _ => none
+instance : Coe Literal (Option TypedLiteral) where coe := Literal.toTyped?
+instance : Coe TypedLiteral Literal where coe := Literal.Typed
+
+def Literal.toLanguageTaggedString? : Literal → (Option LanguageTaggedStringLiteral)
+  | Literal.LanguageTaggedString l => some l
+  | _ => none
+instance : Coe Literal (Option LanguageTaggedStringLiteral) where coe := Literal.toLanguageTaggedString?
+instance : Coe LanguageTaggedStringLiteral Literal where coe := Literal.LanguageTaggedString
+
+-- FIXME: This is to help along nested optionals
+-- see https://leanprover.zulipchat.com/#narrow/stream/113488-general/topic/.E2.9C.94.20Coercing.20recursive.20.60Option.60s/near/422643899
+instance [Coe TypedLiteral (Option α)] : Coe Literal (Option α) where
+  coe a := match (a: Option TypedLiteral) with
+    | some l => l
+    | _ => none
+
+def Int.toTypedLiteral (i: Int): TypedLiteral := ⟨toString i, XSD.integer⟩
+instance : Coe Int TypedLiteral where coe := Int.toTypedLiteral
+
+def TypedLiteral.toInt? (literal: TypedLiteral): Option Int :=
+  if literal.datatype == XSD.integer then String.toInt? literal.value else none
+instance : Coe TypedLiteral (Option Int) where coe := TypedLiteral.toInt?
+
+theorem stringToIntRoundtrip (x: Int) : (String.toInt? (toString x)) = some x := by sorry
+
+-- theorem stringToIntRoundtrip (x: Int) (i: String.Pos) (h1: y = toString x) (h2: i. ≤ y.length) (h3: i ≥ 0) : (String.toInt? (y.)) = some x := by
+--   simp [String.toInt?]
+--   induction x
+--   case zero => exact rfl
+--   case succ x ih => exact ih
+
+-- theorem isNatRoundTrip (x: Nat) : (String.isNat (toString x)) = true := by
+--   cases x
+--   case zero => exact rfl
+--   case succ x ih => simp [toString, Nat.repr, String.isNat]
+  -- simp [ toString, Nat.repr ]
+
+  -- simp [toString, Nat.repr, Nat.toDigits, Nat.toDigitsCore, Nat.digitChar, Char.ofNat, String.utf8ByteSize, Nat.isValidChar, String.isNat, Char.isDigit, String.all, String.isEmpty, String.endPos, List.asString, Nat.toDigits, Nat.toDigitsCore, Nat.digitChar, Char.ofNat, String.utf8ByteSize, Nat.isValidChar, String.utf8ByteSize.go, Char.ofNatAux, UInt32.size]
+  -- simp
+  -- exact rfl
+
+
+  -- search_proof
+  -- simp [String.isNat, Char.isDigit, String.all, String.isEmpty, String.endPos, List.asString, Nat.toDigits, Nat.toDigitsCore, Nat.digitChar, Char.ofNat, String.utf8ByteSize, Nat.isValidChar];
+  -- decide
+  -- exact ⟨by decide, by decide ⟩
+  -- cases toString x <;>
+  -- simp [toString ]
+  -- simp [toString, String.all ]
+  -- simp [String.isEmpty ]
+  -- simp [String.all ]
+  -- unfold  String.isEmpty
+  -- simp [toString, toString ]
+  -- simp [String.all, toString ]
+  -- unfold  String.all
+  -- unfold  toString
+  -- cases x <;>  decide
+  -- cases toString  x
+  -- cases toString x <;>  simp!
+  -- constructor <;>  intro
+  --  trivial
+  -- constructor <;> intro  h
+  -- constructor <;>  simp
+  --  constructor
+  -- cases  x
+  -- suggest_tactics
+  -- suggest_tactics
+  -- induction x
+  -- case zero => exact rfl
+  -- case succ x ih => simp [toString, Nat.repr]
+
+  -- simp [String.isNat, Char.isDigit];
+  -- -- simp [String.isNat, toString, Nat.repr, String.isEmpty, String.endPos, List.asString, Nat.toDigits, Nat.toDigitsCore, Nat.digitChar, Char.ofNat, String.utf8ByteSize, Nat.isValidChar, ]
+
+  -- -- simp [String.isNat, toString, Nat.repr, String.isEmpty, String.endPos, List.asString, Nat.toDigits, Nat.toDigitsCore, Nat.digitChar, Char.ofNat, String.utf8ByteSize, Nat.isValidChar, ]
+
+  -- induction x
+  -- case zero => exact rfl
+  -- case succ x ih => exact ih
+
+-- theorem stringToNatRoundtrip (x: Nat) : (String.toNat? (toString x)) = some x := by
+--   simp [String.toNat?]
+--   induction x
+--   case zero => exact rfl
+--   case succ x ih =>
+
+  -- cases (String.toNat? (toString x)) with
+  --   | none => exact rfl
+  --   | some y => exact ih
+  -- exact (stringToNatRoundtrip x)
+
+
+theorem intInverse (x: Int) : (TypedLiteral.toInt? (Int.toTypedLiteral x)) = some x := by
+  simp [TypedLiteral.toInt?, Int.toTypedLiteral]
+  exact (stringToIntRoundtrip x)
+
+def Bool.toTypedLiteral (i: Bool): TypedLiteral := ⟨toString i, XSD.boolean⟩
+instance : Coe Bool TypedLiteral where coe := Bool.toTypedLiteral
+
+def TypedLiteral.toBool? (literal: TypedLiteral): Option Bool :=
+  if literal.datatype == XSD.boolean then
+    match literal.value.toLower with
+    | "true" | "1" => some true
+    | "false" | "0" => some false
+    | _ => none
+  else none
+instance : Coe TypedLiteral (Option Bool) where coe := TypedLiteral.toBool?
+
+theorem boolInverse (x: Bool) : (TypedLiteral.toBool? (Bool.toTypedLiteral x)) = some x := by cases x <;> exact rfl
+
+instance : Coe Float TypedLiteral where coe s := ⟨toString s, XSD.float⟩
+-- FIXME: Implement reverse direction
+
+def String.toTypedLiteral (s: String): TypedLiteral := ⟨s, XSD.string⟩
+instance : Coe String TypedLiteral where coe := String.toTypedLiteral
+
+def TypedLiteral.toString? (literal: TypedLiteral): Option String :=
+  if literal.datatype == XSD.string then some literal.value else none
+instance : Coe TypedLiteral (Option String) where coe := TypedLiteral.toString?
+
+theorem stringInverse (x: String) : (TypedLiteral.toString? (String.toTypedLiteral x)) = some x := by exact rfl
+
+instance : Coe UInt8 TypedLiteral  where coe s := ⟨toString s, XSD.integer⟩
+instance : Coe UInt16 TypedLiteral where coe s := ⟨toString s, XSD.integer⟩
+instance : Coe UInt32 TypedLiteral where coe s := ⟨toString s, XSD.integer⟩
+instance : Coe UInt64 TypedLiteral where coe s := ⟨toString s, XSD.integer⟩
