lakefile.lean
@@ -3,9 +3,14 @@ open System Lake DSL
 
 package RustFFI
 
+lean_lib lib
+
 @[default_target]
 lean_exe ffi where
+  moreLinkArgs := #["-L./.lake/packages/LeanCopilot/.lake/build/lib", "-lctranslate2"]
   root := `Main
+
+require LeanCopilot from git "https://github.com/lean-dojo/LeanCopilot.git" @ "v1.1.1"
 
 extern_lib some_rust_lib (pkg : NPackage _package.name) := do
   proc { cmd := "cargo", args := #["build", "--release"], cwd := pkg.dir }
