lib/NamedNode.lean
@@ -1,0 +1,3 @@
+structure NamedNode where
+  iri : String
+deriving Repr, DecidableEq
