lib/RDF.lean
@@ -1,97 +1,97 @@
-class NamedNode (a : Type) where
-  namedNode : String → a
+-- class NamedNode (a : Type) where
+--   namedNode : String → a
 
-inductive Subject where
-  | NamedNode : String → Subject
-  | BlankNode : String → Subject
-deriving Repr
+-- inductive Subject where
+--   | NamedNode : String → Subject
+--   | BlankNode : String → Subject
+-- deriving Repr
 
-instance : ToString Subject where
-  toString s := match s with
-  | Subject.NamedNode s => s
-  | Subject.BlankNode s => s
+-- instance : ToString Subject where
+--   toString s := match s with
+--   | Subject.NamedNode s => s
+--   | Subject.BlankNode s => s
 
-inductive Predicate where
-  | NamedNode : String → Predicate
-deriving Repr
+-- inductive Predicate where
+--   | NamedNode : String → Predicate
+-- deriving Repr
 
-instance : ToString Predicate where
-  toString s := match s with
-  | Predicate.NamedNode s => s
+-- instance : ToString Predicate where
+--   toString s := match s with
+--   | Predicate.NamedNode s => s
 
-inductive Literal where
-  | Language : String → Literal
-  | DataTyped : String → String → Literal
+-- inductive Literal where
+--   | Language : String → Literal
+--   | DataTyped : String → String → Literal
 
-inductive Object where
-  | NamedNode : String → Object
-  | BlankNode : String → Object
-  | Literal : String → Object
-deriving Repr
+-- inductive Object where
+--   | NamedNode : String → Object
+--   | BlankNode : String → Object
+--   | Literal : String → Object
+-- deriving Repr
 
--- TODO: Mirror the rust literal coercions here.
+-- -- TODO: Mirror the rust literal coercions here.
 
-instance : Coe Int Literal where
-  coe s := Literal.DataTyped (toString s) "http://www.w3.org/2001/XMLSchema#integer"
+-- instance : Coe Int Literal where
+--   coe s := Literal.DataTyped (toString s) "http://www.w3.org/2001/XMLSchema#integer"
 
-instance : Coe Bool Literal where
-  coe s := Literal.DataTyped (toString s) "http://www.w3.org/2001/XMLSchema#boolean"
+-- instance : Coe Bool Literal where
+--   coe s := Literal.DataTyped (toString s) "http://www.w3.org/2001/XMLSchema#boolean"
 
-instance : Coe Float Literal where
-  coe s := Literal.DataTyped (toString s) "http://www.w3.org/2001/XMLSchema#float"
-
-instance : Coe String Literal where
-  coe s := Literal.DataTyped s "http://www.w3.org/2001/XMLSchema#string"
-
--- instance : Coe String Object where
---   coe s := Object.Literal s
-
+-- instance : Coe Float Literal where
+--   coe s := Literal.DataTyped (toString s) "http://www.w3.org/2001/XMLSchema#float"
 
 -- instance : Coe String Literal where
---   coe s := Literal.DataTyped s ""
+--   coe s := Literal.DataTyped s "http://www.w3.org/2001/XMLSchema#string"
 
-instance : ToString Object where
-  toString s := match s with
-  | Object.NamedNode s => s
-  | Object.BlankNode s => s
-  | Object.Literal s => s
+-- -- instance : Coe String Object where
+-- --   coe s := Object.Literal s
 
-inductive Term where
-  | NamedNode : String → Term
-  | BlankNode : String → Term
-  | Literal : String → Term
-  | Variable : String → Term
-  | DefaultGraph
-deriving Inhabited, Repr
 
-instance : ToString Term where
-  toString s := match s with
-  | Term.NamedNode s => s
-  | Term.BlankNode s => s
-  | Term.Literal s => s
-  | Term.Variable s => s
-  | Term.DefaultGraph => "DefaultGraph"
+-- -- instance : Coe String Literal where
+-- --   coe s := Literal.DataTyped s ""
 
-structure Triple where
-  subject : Subject
-  predicate : Predicate
-  object : Object
-deriving Repr
+-- instance : ToString Object where
+--   toString s := match s with
+--   | Object.NamedNode s => s
+--   | Object.BlankNode s => s
+--   | Object.Literal s => s
 
-instance : ToString Triple where
-  toString t := "(" ++ toString t.subject ++ ", " ++ toString t.predicate ++ ", " ++ toString t.object ++ ")"
+-- inductive Term where
+--   | NamedNode : String → Term
+--   | BlankNode : String → Term
+--   | Literal : String → Term
+--   | Variable : String → Term
+--   | DefaultGraph
+-- deriving Inhabited, Repr
 
-instance : Coe Subject Term where
-  coe s := match s with
-  | Subject.NamedNode s => Term.NamedNode s
-  | Subject.BlankNode s => Term.BlankNode s
+-- instance : ToString Term where
+--   toString s := match s with
+--   | Term.NamedNode s => s
+--   | Term.BlankNode s => s
+--   | Term.Literal s => s
+--   | Term.Variable s => s
+--   | Term.DefaultGraph => "DefaultGraph"
 
-instance : Coe Predicate Term where
-  coe s := match s with
-  | Predicate.NamedNode s => Term.NamedNode s
+-- structure Triple where
+--   subject : Subject
+--   predicate : Predicate
+--   object : Object
+-- deriving Repr
 
-instance : Coe Object Term where
-  coe s := match s with
-  | Object.NamedNode s => Term.NamedNode s
-  | Object.BlankNode s => Term.BlankNode s
-  | Object.Literal s => Term.Literal s
+-- instance : ToString Triple where
+--   toString t := "(" ++ toString t.subject ++ ", " ++ toString t.predicate ++ ", " ++ toString t.object ++ ")"
+
+-- instance : Coe Subject Term where
+--   coe s := match s with
+--   | Subject.NamedNode s => Term.NamedNode s
+--   | Subject.BlankNode s => Term.BlankNode s
+
+-- instance : Coe Predicate Term where
+--   coe s := match s with
+--   | Predicate.NamedNode s => Term.NamedNode s
+
+-- instance : Coe Object Term where
+--   coe s := match s with
+--   | Object.NamedNode s => Term.NamedNode s
+--   | Object.BlankNode s => Term.BlankNode s
+--   | Object.Literal s => Term.Literal s
